disk-betree/ImplIO.i.dfy
@@ -1,0 +1,219 @@
+include "Impl.i.dfy"
+
+module ImplIO { 
+  import opened Impl
+  import opened MainDiskIOHandler
+  import opened NativeTypes
+  import opened Options
+  import IS = ImplState
+
+  method getFreeLba(s: ImplVariables, len: uint64)
+  returns (loc : Option<BC.Location>)
+  requires s.Ready?
+  requires IS.WFVars(s)
+  requires len <= LBAType.BlockSize()
+  ensures loc.Some? ==> BC.ValidLocationForNode(loc.value)
+  ensures loc.Some? ==> BC.ValidAllocation(IS.IVars(s), loc.value)
+  ensures loc.Some? ==> loc.value.len == len
+  {
+    var persistent': map<uint64, (Option<BC.Location>, seq<IS.Reference>)> := s.persistentIndirectionTable.ToMap();
+    var persistent: map<uint64, BC.Location> := map ref | ref in persistent' && persistent'[ref].0.Some? :: persistent'[ref].0.value;
+
+    var ephemeral': map<uint64, (Option<BC.Location>, seq<IS.Reference>)> := s.ephemeralIndirectionTable.ToMap();
+    var ephemeral := map ref | ref in ephemeral' && ephemeral'[ref].0.Some? :: ephemeral'[ref].0.value;
+
+    var frozen: Option<map<uint64, BC.Location>> := None;
+    if (s.frozenIndirectionTable.Some?) {
+      var m := s.frozenIndirectionTable.value.ToMap();
+      var frozen' := m;
+      frozen := Some(map ref | ref in frozen' && frozen'[ref].0.Some? :: frozen'[ref].0.value);
+    }
+
+    if i: uint64 :| (
+      && i as int * LBAType.BlockSize() as int < 0x1_0000_0000_0000_0000
+      && var l := i * LBAType.BlockSize();
+      && BC.ValidLBAForNode(l)
+      && (forall ref | ref in persistent :: persistent[ref].addr != l)
+      && (forall ref | ref in ephemeral :: ephemeral[ref].addr != l)
+      && (frozen.Some? ==> (forall ref | ref in frozen.value :: frozen.value[ref].addr != l))
+      && (forall id | id in s.outstandingBlockWrites :: s.outstandingBlockWrites[id].loc.addr != l)
+    ) {
+      loc := Some(LBAType.Location(i * LBAType.BlockSize(), len));
+
+      assert IS.IVars(s).persistentIndirectionTable.locs == persistent;
+      assert IS.IVars(s).ephemeralIndirectionTable.locs == ephemeral;
+      assert IS.IVars(s).frozenIndirectionTable.Some? ==>
+          IS.IVars(s).frozenIndirectionTable.value.locs == frozen.value;
+    } else {
+      loc := None;
+    }
+  }
+
+  method RequestWrite(io: DiskIOHandler, loc: LBAType.Location, sector: IS.Sector)
+  returns (id: Option<D.ReqId>)
+  requires IS.WFSector(sector)
+  requires sector.SectorBlock? ==> BT.WFNode(IS.INode(sector.block))
+  requires sector.SectorBlock? ==> Marshalling.CappedNode(sector.block)
+  requires io.initialized()
+  requires LBAType.ValidLocation(loc)
+  modifies io
+  ensures ImplADM.M.ValidDiskOp(io.diskOp())
+  ensures id.Some? ==> ImplADM.M.IDiskOp(io.diskOp()) == SD.ReqWriteOp(id.value, SD.ReqWrite(loc, IS.ISector(sector)))
+  ensures id.None? ==> ImplADM.M.IDiskOp(io.diskOp()) == SD.NoDiskOp
+  {
+    Marshalling.reveal_parseCheckedSector();
+    ImplADM.M.reveal_IBytes();
+    ImplADM.M.reveal_ValidCheckedBytes();
+    ImplADM.M.reveal_Parse();
+    D.reveal_ChecksumChecksOut();
+
+    var bytes := Marshalling.MarshallCheckedSector(sector);
+    if (bytes == null || bytes.Length as uint64 != loc.len) {
+      id := None;
+    } else {
+      var i := io.write(loc.addr, bytes);
+      id := Some(i);
+
+      //assert ImplADM.M.ValidReqWrite(io.diskOp().reqWrite);
+    }
+  }
+
+  method FindLocationAndRequestWrite(s: ImplVariables, io: DiskIOHandler, sector: IS.Sector)
+  returns (id: Option<D.ReqId>, loc: Option<LBAType.Location>)
+  requires IS.WFVars(s)
+  requires s.Ready?
+  requires IS.WFSector(sector)
+  requires sector.SectorBlock? ==> BT.WFNode(IS.INode(sector.block))
+  requires sector.SectorBlock? ==> Marshalling.CappedNode(sector.block)
+  requires io.initialized()
+  modifies io
+  ensures ImplADM.M.ValidDiskOp(io.diskOp())
+  ensures id.Some? ==> loc.Some?
+  ensures id.Some? ==> LBAType.ValidLocation(loc.value)
+  ensures id.Some? ==> BC.ValidAllocation(old(IS.IVars(s)), loc.value)
+  ensures id.Some? ==> loc.value.addr != BC.IndirectionTableLBA()
+  ensures id.Some? ==> ImplADM.M.IDiskOp(io.diskOp()) == SD.ReqWriteOp(id.value, SD.ReqWrite(loc.value, IS.ISector(sector)))
+  ensures id.None? ==> ImplADM.M.IDiskOp(io.diskOp()) == SD.NoDiskOp
+  {
+    Marshalling.reveal_parseCheckedSector();
+    ImplADM.M.reveal_IBytes();
+    ImplADM.M.reveal_ValidCheckedBytes();
+    ImplADM.M.reveal_Parse();
+    D.reveal_ChecksumChecksOut();
+
+    var bytes := Marshalling.MarshallCheckedSector(sector);
+    if (bytes == null) {
+      id := None;
+      loc := None;
+    } else {
+      var len := bytes.Length as uint64;
+      loc := getFreeLba(s, len);
+      if (loc.Some?) {
+        var i := io.write(loc.value.addr, bytes);
+        id := Some(i);
+      } else {
+        id := None;
+      }
+    }
+  }
+
+  method RequestRead(io: DiskIOHandler, loc: LBAType.Location)
+  returns (id: D.ReqId)
+  requires io.initialized()
+  requires LBAType.ValidLocation(loc)
+  modifies io
+  ensures ImplADM.M.ValidDiskOp(io.diskOp())
+  ensures ImplADM.M.IDiskOp(io.diskOp()) == SD.ReqReadOp(id, SD.ReqRead(loc))
+  {
+    id := io.read(loc.addr, loc.len);
+  }
+
+  lemma LemmaIndirectionTableLBAValid()
+  ensures ImplADM.M.ValidAddr(BC.IndirectionTableLBA())
+  {
+    LBAType.reveal_ValidAddr();
+    assert BC.IndirectionTableLBA() as int == 0 * ImplADM.M.BlockSize();
+  }
+
+  method PageInIndirectionTableReq(k: ImplConstants, s: ImplVariables, io: DiskIOHandler)
+  returns (s': ImplVariables)
+  requires IS.WFVars(s)
+  requires io.initialized();
+  requires s.Unready?
+  modifies io
+  ensures IS.WFVars(s')
+  ensures ImplADM.M.Next(Ik(k), IS.IVars(s), IS.IVars(s'), UI.NoOp, io.diskOp())
+  {
+    if (s.outstandingIndirectionTableRead.None?) {
+      LemmaIndirectionTableLBAValid();
+      var id := RequestRead(io, BC.IndirectionTableLocation());
+      s' := IS.Unready(Some(id), s.syncReqs);
+
+      assert stepsBC(k, IS.IVars(s), IS.IVars(s'), UI.NoOp, io, BC.PageInIndirectionTableReqStep);
+    } else {
+      s' := s;
+      assert noop(k, IS.IVars(s), IS.IVars(s'));
+      print "PageInIndirectionTableReq: request already out\n";
+    }
+  }
+
+  method PageInReq(k: ImplConstants, s: ImplVariables, io: DiskIOHandler, ref: BC.Reference)
+  returns (s': ImplVariables)
+  requires io.initialized();
+  requires s.Ready?
+  requires IS.WFVars(s)
+  requires BBC.Inv(k, IS.IVars(s))
+  requires ref in IS.IIndirectionTable(s.ephemeralIndirectionTable).locs
+  requires ref !in s.cache
+  modifies io
+  ensures IS.WFVars(s')
+  ensures ImplADM.M.Next(Ik(k), IS.IVars(s), IS.IVars(s'), UI.NoOp, io.diskOp())
+  {
+    if (BC.OutstandingRead(ref) in s.outstandingBlockReads.Values) {
+      s' := s;
+      assert noop(k, IS.IVars(s), IS.IVars(s'));
+      print "giving up; already an outstanding read for this ref\n";
+    } else {
+      var lbaGraph := s.ephemeralIndirectionTable.Get(ref);
+      assert lbaGraph.Some?;
+      var (lba, _) := lbaGraph.value;
+      assert lba.Some?;
+      assert BC.ValidLocationForNode(lba.value);
+      var id := RequestRead(io, lba.value);
+      s' := s.(outstandingBlockReads := s.outstandingBlockReads[id := BC.OutstandingRead(ref)]);
+
+      assert BC.PageInReq(k, IS.IVars(s), IS.IVars(s'), ImplADM.M.IDiskOp(io.diskOp()), ref);
+      assert stepsBC(k, IS.IVars(s), IS.IVars(s'), UI.NoOp, io, BC.PageInReqStep(ref));
+    }
+  }
+
+  lemma INodeRootEqINodeForEmptyRootBucket(node: IS.Node)
+  requires IS.WFNode(node)
+  ensures IS.INodeRoot(node, TTT.EmptyTree) == IS.INode(node);
+  {
+    assume false;
+  }
+  /*{
+    assert BT.AddMessagesToBuckets(node.pivotTable, |node.buckets|, SSTable.ISeq(node.buckets),
+          map[]) == SSTable.ISeq(node.buckets);
+  }*/
+
+  /*lemma LemmaPageInBlockCacheSet(s: ImplVariables, ref: BT.G.Reference, node: IS.Node)
+  requires IS.WFVars(s)
+  requires s.Ready?
+  requires ref !in s.cache
+  requires IS.WFNode(node)
+  ensures IS.ICache(s.cache, s.rootBucket)[ref := IS.INode(node)]
+       == IS.ICache(s.cache[ref := node], s.rootBucket);
+  {
+    if (ref == BT.G.Root()) {
+      //assert TTT.I(rootBucket) == map[];
+      //assert BT.AddMessagesToBuckets(node.pivotTable, |node.buckets|, SSTable.ISeq(node.buckets),
+      //    map[]) == IS.INode(node).buckets;
+      INodeRootEqINodeForEmptyRootBucket(node);
+      assert IS.INodeRoot(node, s.rootBucket) == IS.INode(node);
+    }
+    assert IS.INodeForRef(s.cache[ref := node], ref, s.rootBucket) == IS.INode(node);
+    assert IS.ICache(s.cache[ref := node], s.rootBucket)[ref] == IS.INode(node);
+  }*/
+}
